providers/evercrypt/EverCrypt.Helpers.fsti
@@ -23,3 +23,5 @@ let uint8_p = B.buffer uint8_t
 let uint16_p = B.buffer uint16_t
 let uint32_p = B.buffer uint32_t
 let uint64_p = B.buffer uint64_t
+
+let uint8_pl (l:nat) = p:uint8_p {B.length p = l}
